All.thy
@@ -1,7 +1,7 @@
 section \<open>Convenience theory for loading all others\<close>
 
 theory All
-  imports Laws Classical_Extra Teleport Experiments
+  imports Laws Classical_Extra Teleport Laws_Complement_Quantum
 begin
 
 end
