Axioms_Complement.thy
@@ -4,5 +4,14 @@ theory Axioms_Complement
   imports Laws
 begin
 
+typedecl ('a, 'b) complement_domain
+instance complement_domain :: (domain, domain) domain..
+
+axiomatization where 
+  complement_exists: \<open>register F \<Longrightarrow> \<exists>G :: ('a, 'b) complement_domain update \<Rightarrow> 'b update. compatible F G \<and> iso_register (F;G)\<close> for F :: \<open>'a::domain update \<Rightarrow> 'b::domain update\<close>
+
+axiomatization where complement_unique: \<open>compatible F G \<Longrightarrow> iso_register (F;G) \<Longrightarrow> compatible F H \<Longrightarrow> iso_register (F;H)
+          \<Longrightarrow> equivalent_registers G H\<close> 
+    for F :: \<open>'a::domain update \<Rightarrow> 'b::domain update\<close> and G :: \<open>'g::domain update \<Rightarrow> 'b update\<close> and H :: \<open>'h::domain update \<Rightarrow> 'b update\<close>
 
 end
